src/cbor/pulse/raw/CBOR.Pulse.Raw.Format.MixedList.fsti
@@ -1,0 +1,3 @@
+module CBOR.Pulse.Raw.Format.MixedList
+
+val cbor_raw_mixed_list ([@@@strictly_positive] t: Type0) : Type0
